Finished implem of spec of Argon, debugging to come

specs/Spec.Argon2i.fst
@@ -2,17 +2,17 @@ module Spec.Argon2i
 
 #reset-options "--z3rlimit 100 --max_fuel 0"
 
-open FStar.Mul
+let ( *$ ) = FStar.Mul.(( * ))
 open Spec.Lib.IntTypes
 open Spec.Lib.IntSeq
 open Spec.Lib.RawIntTypes
 
-let version_number : uint8 = u8 0x13
-let argon_type : nat = 1
-let size_of_block = 1024
+let version_number : uint8 = assert_norm (0x13 < maxint (U8));u8 0x13
+let argon_type = 1
+let block_size = 1024
+let line_size = 128
 
-val h : a_len:size_nat{0 < a_len /\ a_len <=max_size_t - 2 * Spec.Blake2b.bytes_in_block} -> a:lbytes a_len -> nn:size_nat{1 <= nn /\ nn <= 64} -> Tot (lbytes nn)
-
+val h : a_len:size_nat{0 < a_len /\ a_len <=max_size_t - 2 *$line_size} -> a:lbytes a_len -> nn:size_nat{1 <= nn /\ nn <= 64} -> Tot (lbytes nn)
 let h a_len a nn =
   let null_list = [] in
   let null_key : lbytes 0 = assert_norm (List.Tot.length null_list = 0); createL #uint8 null_list in
@@ -25,21 +25,21 @@ val step1 :
   m:size_nat ->
   iterations:size_nat ->
   x_len:size_nat -> x:lbytes x_len ->
-  k_len:size_nat{k_len + p_len + s_len + x_len + 11*4 <= max_size_t - 2 * Spec.Blake2b.bytes_in_block} -> k:lbytes k_len ->
+  k_len:size_nat{k_len + p_len + s_len + x_len + 11*$4 <= max_size_t - 2*$line_size} -> k:lbytes k_len ->
   Tot (lbytes 64)
-
 let step1 p_len p s_len s lanes t_len m iterations x_len x k_len k =
-  let lanes_as_word = uint_to_bytes_le (u32 lanes) in
-  let t_len_as_word = uint_to_bytes_le (u32 t_len) in
-  let m_as_word = uint_to_bytes_le (u32 m) in
-  let iterations_as_word = uint_to_bytes_le (u32 iterations) in
-  let v_as_word = uint_to_bytes_le (to_u32 version_number) in
-  let argon_type_as_word = uint_to_bytes_le (u32 argon_type) in
-  let p_len_as_word = uint_to_bytes_le (u32 p_len) in
-  let s_len_as_word = uint_to_bytes_le (u32 s_len) in
-  let k_len_as_word = uint_to_bytes_le (u32 k_len) in
-  let x_len_as_word = uint_to_bytes_le (u32 x_len) in
-  let blake2_argument_size : size_nat = 11 * 4 + p_len + k_len + s_len + x_len in
+  (* This is basically a big concatenation *)
+  let lanes_as_word = uint_to_bytes_le #U32 (u32 lanes) in
+  let t_len_as_word = uint_to_bytes_le #U32 (u32 t_len) in
+  let m_as_word = uint_to_bytes_le #U32 (u32 m) in
+  let iterations_as_word = uint_to_bytes_le #U32 (u32 iterations) in
+  let v_as_word = uint_to_bytes_le #U32 (to_u32 #U8 version_number) in
+  let argon_type_as_word = uint_to_bytes_le #U32 (u32 argon_type) in
+  let p_len_as_word = uint_to_bytes_le #U32 (u32 p_len) in
+  let s_len_as_word = uint_to_bytes_le #U32 (u32 s_len) in
+  let k_len_as_word = uint_to_bytes_le #U32 (u32 k_len) in
+  let x_len_as_word = uint_to_bytes_le #U32 (u32 x_len) in
+  let blake2_argument_size : size_nat = 11*$4 + p_len + k_len + s_len + x_len in
   let blake2_argument = create blake2_argument_size (u8 0) in
   let blake2_argument = update_slice blake2_argument 0 4 lanes_as_word in
   let blake2_argument = update_slice blake2_argument 4 8 t_len_as_word in
@@ -63,18 +63,17 @@ let step1 p_len p s_len s lanes t_len m iterations x_len x k_len k =
 
 let ceil_32 (x:size_nat) : Tot size_nat = if x % 32 = 0 then x / 32 else x / 32  + 1
 
-let compute_variable_length_output_size (t_len:size_nat{t_len + 64 <= size_of_block}) : Tot (result:size_nat{result <= size_of_block}) =
+let compute_variable_length_output_size (t_len:size_nat{t_len + 64 <= block_size}) : Tot (result:size_nat{result <= block_size}) =
   if t_len <= 64 then t_len else
     let r = (ceil_32 t_len) - 2 in
-    32 * r + 64
+    32*$r + 64
 
-val h' : t_len:size_nat{1 <= t_len /\ t_len + 64 <= size_of_block} -> x_len:size_nat{x_len + 4 <= max_size_t - 2 * Spec.Blake2b.bytes_in_block} -> x:lbytes x_len -> Tot (lbytes ( compute_variable_length_output_size t_len))
-
+val h' : t_len:size_nat{1 <= t_len /\ t_len + 64 <= block_size} -> x_len:size_nat{x_len + 4 <= max_size_t - 2*$line_size} -> x:lbytes x_len -> Tot (lbytes ( compute_variable_length_output_size t_len))
 
 let h' t_len x_len x =
   let t_with_x_len : size_nat = x_len + 4 in
   let t_with_x = create t_with_x_len (u8 0) in
-  let t_with_x = update_slice t_with_x 0 4 (uint_to_bytes_le (u32 t_len)) in
+  let t_with_x = update_slice t_with_x 0 4 (uint_to_bytes_le #U32 (u32 t_len)) in
   let t_with_x = update_slice t_with_x 4 t_with_x_len x in
   if t_len <= 64 then
     h t_with_x_len t_with_x t_len
@@ -86,12 +85,12 @@ let h' t_len x_len x =
     let (output,vlast) = repeati (r-1) (fun i (output,vprevious) ->
       let i = i + 1 in (* we did the first iteration outside the loop *)
       let v = h 64 vprevious 64 in
-      (update_slice output (i * 32) ((i+1)*32) (sub v 0 32),v)
+      (update_slice output (i*$32) ((i+1)*$32) (sub v 0 32),v)
     ) (output,v1)
     in
-    update_slice output (r * 32) ((r*32)+64) vlast
+    update_slice output (r*$32) ((r*$32)+64) vlast
 
-let low_bits x = to_u64 (to_u32 #U64 x)
+let low_bits x = to_u64 #U32 (to_u32 #U64 x)
 
 type idx = idx:size_nat{idx <= 15}
 
@@ -108,11 +107,11 @@ let g (a:uint64) (b:uint64) (c:uint64) (d:uint64) =
 
 let permutation_matrix_index_to_offset (i:idx) : Tot size_nat =
    if i % 2 = 0 then
-     8*((i/2)+1)
+     8*$((i/2)+1)
    else
-     8*(i/2)
+     8*$(i/2)
 
-let apply_g (v:lbytes 128) (i1:idx) (i2:idx) (i3:idx) (i4:idx) : Tot (lbytes 128) =
+let apply_g (v:lbytes 128) (i1:idx) (i2:idx) (i3:idx) (i4:idx) : Tot (lbytes line_size) =
   let o1 = permutation_matrix_index_to_offset i1 in
   let o2 = permutation_matrix_index_to_offset i2 in
   let o3 = permutation_matrix_index_to_offset i3 in
@@ -128,8 +127,7 @@ let apply_g (v:lbytes 128) (i1:idx) (i2:idx) (i3:idx) (i4:idx) : Tot (lbytes 128
   let v = update_slice v o4 (o4 + 8) (uint_to_bytes_be d) in
   v
 
-val argon_permute : input: lbytes 128 -> Tot (lbytes 128)
-
+val argon_permute : input: lbytes line_size -> Tot (lbytes line_size)
 let argon_permute input =
   let v : lbytes 128 = apply_g input 0 4 8 12 in
   let v : lbytes 128 = apply_g v 1 5 9  13 in
@@ -142,39 +140,41 @@ let argon_permute input =
   v
 
 
-
-let xor_matrices (x:lbytes 1024) (y:lbytes 1024) : Tot (lbytes 1024) =
-  let r = create 1024 (u8 0) in
-  repeati (1024 / 8) (fun i r ->
-    update_slice r (8*i) (8*(i+1)) (uint_to_bytes_be (
-      (uint_from_bytes_be #U64 (sub x (8*i) 8)) ^. (uint_from_bytes_be #U64 (sub y (8*i) 8))
+let xor_matrices (x:lbytes block_size) (y:lbytes block_size) : Tot (lbytes block_size) =
+  let r = create block_size (u8 0) in
+  repeati (block_size / 8) (fun i r ->
+    update_slice r (8*$i) (8*$(i+1)) (uint_to_bytes_be (
+      (uint_from_bytes_be #U64 (sub x (8*$i) 8)) ^. (uint_from_bytes_be #U64 (sub y (8*$i) 8))
     ))
   ) r
 
-let extract_column_from_matrix (r: lbytes 1024) (j:size_nat{j < 8}) : Tot (lbytes 128) =
-  let output = create 128 (u8 0) in
+let extract_column_from_matrix (r: lbytes block_size) (j:size_nat{j < 8}) : Tot (lbytes line_size) =
+  let output : lbytes line_size = create line_size (u8 0) in
   let output = repeati 8 (fun i output ->
-    update_slice output (i*16) ((i+1)*16) (sub r (i*128 + j*16) 16)
+    let r_offset : size_nat = i*$line_size + j*$16 in
+    update_slice output (i*$16) ((i+1)*$16) (sub r r_offset 16)
   ) output
   in
   output
 
-let update_column_to_matrix (col:lbytes 128) (r:lbytes 1024) (j:size_nat{j < 8}) : Tot (lbytes 1024) =
-  repeati 8 (fun i r ->
-    update_slice r (i*128 + j*16) (i*128 + (j+1)*16) (sub col (i*16) 16)
+let update_column_to_matrix (col:lbytes line_size) (r:lbytes block_size) (j:size_nat{j < 8}) : Tot (lbytes block_size) =
+  repeati 8 (fun i (r:lbytes block_size) ->
+    let r_offset = i*$line_size + j*$16 in
+     update_slice r r_offset (r_offset + 16) (sub col (i*$16) 16)
   ) r
 
-let argon_compress (x:lbytes 1024) (y:lbytes 1024) : Tot (lbytes 1024) =
-  let r = create 1024 (u8 0) in
+let argon_compress (x:lbytes block_size) (y:lbytes block_size) : Tot (lbytes block_size) =
+  let r : lbytes block_size = create block_size (u8 0) in
   let r = xor_matrices x y in
   (* permute rows *)
-  let q = repeati (1024 / 128) (fun i r ->
-    let row = sub r (128*i) 128 in
+  let q = repeati 8 (fun i r ->
+    assert_norm (0 <= i /\ i < 8);
+    let row : lbytes line_size = sub r (line_size*$i) line_size in
     let row = argon_permute row in
-    update_slice r (128*i) (128*(i+1)) row
+    update_slice r (line_size*$i) (line_size*$(i+1)) row
   ) r in
   (* permute columns *)
-  let z = repeati (1024 / 128) (fun j q ->
+  let z = repeati 8 (fun j q ->
     let col = extract_column_from_matrix q j in
     let col = argon_permute col in
     update_column_to_matrix col q j
@@ -183,19 +183,19 @@ let argon_compress (x:lbytes 1024) (y:lbytes 1024) : Tot (lbytes 1024) =
 
 
 
-let fill_block (d_len: size_nat{d_len <= size_of_block}) (d: lbytes d_len) : Tot (lbytes size_of_block) =
-  let output = create size_of_block (u8 0) in
+let fill_block (d_len: size_nat{d_len <= block_size}) (d: lbytes d_len) : Tot (lbytes block_size) =
+  let output = create block_size (u8 0) in
   update_slice output 0 d_len d
 
 #reset-options "--z3rlimit 50 --max_fuel 1"
 
-let block_offset (lanes:size_nat{lanes <> 0}) (columns:size_nat{columns <> 0 /\ columns*lanes*size_of_block <= max_size_t}) (i:size_nat{i<lanes}) (j:size_nat{j<columns}) : Tot (result:size_nat{result <= (lanes * columns - 1) * size_of_block}) =
-   assert (columns * i <= columns * (lanes - 1));
-   assert (columns * i + j <= columns * (lanes - 1) + (columns - 1));
-   assert (columns * i + j <= columns * lanes - 1);
-   size_of_block * (columns * i + j)
+let block_offset (lanes:size_nat{lanes <> 0}) (columns:size_nat{columns <> 0 /\ columns*$lanes*$block_size <= max_size_t}) (i:size_nat{i<lanes}) (j:size_nat{j<columns}) : Tot (result:size_nat{result <= (lanes*$columns - 1)*$block_size}) =
+   assert (columns*$i <= columns*$(lanes - 1));
+   assert (columns*$i + j <= columns*$(lanes - 1) + (columns - 1));
+   assert (columns*$i + j <= columns*$lanes - 1);
+   block_size*$(columns*$i + j)
 
-val step3 : t_len:size_nat{1 <= t_len /\ t_len <= size_of_block - 64} -> lanes:size_nat{lanes >= 1 /\ lanes <= pow2 24 - 1} -> columns:size_nat{1 <= columns /\ lanes * columns * size_of_block <= max_size_t} -> mem: lbytes (lanes * columns * size_of_block) -> h0:lbytes 64 -> Tot (lbytes (lanes * columns * size_of_block))
+val step3 : t_len:size_nat{1 <= t_len /\ t_len <= block_size - 64} -> lanes:size_nat{lanes >= 1 /\ lanes <= pow2 24 - 1} -> columns:size_nat{1 <= columns /\ lanes*$columns*$block_size <= max_size_t} -> mem: lbytes (lanes*$columns*$block_size) -> h0:lbytes 64 -> Tot (lbytes (lanes*$columns*$block_size))
 
 let step3 t_len lanes columns mem h0 =
   repeati lanes (fun i mem ->
@@ -203,15 +203,15 @@ let step3 t_len lanes columns mem h0 =
     let argument_length : size_nat = 64 + 4 + 4 in
     let argument = create argument_length (u8 0) in
     let argument = update_slice argument 0 64 h0 in
-    let argument = update_slice argument (64 + 4) argument_length (uint_to_bytes_le (u32 i)) in
+    let argument = update_slice argument (64 + 4) argument_length (uint_to_bytes_le #U32 (u32 i)) in
     let slice =
       fill_block (compute_variable_length_output_size t_len) (h' t_len argument_length argument)
     in
-    update_slice mem offset (offset + size_of_block) slice
+    update_slice mem offset (offset + block_size) slice
   ) mem
 
 
-val step4 : t_len:size_nat{1 <= t_len /\ t_len <= size_of_block - 64} -> lanes:size_nat{lanes >= 1 /\ lanes <= pow2 24 - 1} -> columns:size_nat{4 <= columns /\ lanes * columns * size_of_block <= max_size_t} -> mem: lbytes (lanes * columns * size_of_block) -> h0:lbytes 64 -> Tot (lbytes (lanes * columns * size_of_block))
+val step4 : t_len:size_nat{1 <= t_len /\ t_len <= block_size - 64} -> lanes:size_nat{lanes >= 1 /\ lanes <= pow2 24 - 1} -> columns:size_nat{4 <= columns /\ lanes*$columns*$block_size <= max_size_t} -> mem: lbytes (lanes*$columns*$block_size) -> h0:lbytes 64 -> Tot (lbytes (lanes*$columns*$block_size))
 
 let step4 t_len lanes columns mem h0 =
   repeati lanes (fun i mem ->
@@ -219,47 +219,114 @@ let step4 t_len lanes columns mem h0 =
     let argument_length : size_nat = 64 + 4 + 4 in
     let argument = create argument_length (u8 0) in
     let argument = update_slice argument 0 64 h0 in
-    let argument = update_slice argument 64 68 (uint_to_bytes_le (u32 1)) in
-    let argument = update_slice argument (64 + 4) argument_length (uint_to_bytes_le (u32 i)) in
+    let argument = update_slice argument 64 68 (uint_to_bytes_le #U32 (u32 1)) in
+    let argument = update_slice argument (64 + 4) argument_length (uint_to_bytes_le #U32 (u32 i)) in
     let slice =
       fill_block (compute_variable_length_output_size t_len) (h' t_len argument_length argument)
     in
-    update_slice mem offset (offset + size_of_block) slice
+    update_slice mem offset (offset + block_size) slice
   ) mem
 
-val step5 : t_len:size_nat{1 <= t_len /\ t_len <= size_of_block - 64} -> lanes:size_nat{lanes >= 1 /\ lanes <= pow2 24 - 1} -> columns:size_nat{4 <= columns /\ lanes * columns * size_of_block <= max_size_t} -> mem: lbytes (lanes * columns * size_of_block) -> Tot (lbytes (lanes * columns * size_of_block))
+val map_indexes : iterations:size_nat -> r:size_nat -> lanes:size_nat -> columns:size_nat -> i:size_nat{i < lanes} -> j:size_nat{j < columns} -> Tot ((size_nat*size_nat))
 
-let step5 t_len lanes columns mem =
-  repeati lanes (fun i (mem: lbytes (lanes*columns*size_of_block)) ->
-    repeati (columns-1) (fun j (mem:lbytes (lanes*columns*size_of_block)) ->
+let map_indexes iterations r lanes columns i j =
+  let slice = j/4 in
+  let segment_length = columns/4 in
+  let g_arg_zero : lbytes block_size = create block_size (u8 0) in
+  let g_arg : lbytes block_size = update_slice g_arg_zero 0 8 (uint_to_bytes_le #U64 (u64 r)) in
+  let g_arg : lbytes block_size = update_slice g_arg 8 16 (uint_to_bytes_le #U64 (u64 i)) in
+  let g_arg : lbytes block_size = update_slice g_arg 16 24 (uint_to_bytes_le #U64 (u64 slice)) in
+  let g_arg : lbytes block_size = update_slice g_arg 24 32 (uint_to_bytes_le #U64 (u64 (lanes*$columns))) in
+  let g_arg : lbytes block_size = update_slice g_arg 32 40 (uint_to_bytes_le #U64 (u64 iterations)) in
+  let g_arg : lbytes block_size = update_slice g_arg 40 48 (uint_to_bytes_le #U64 (u64 argon_type)) in
+  let g_arg : lbytes block_size = update_slice g_arg 48 56 (uint_to_bytes_le #U64 (u64 ((j%4) + 1))) in
+  let result_block : lbytes block_size = argon_compress g_arg_zero g_arg in
+  let j1 = uint_to_nat (uint_from_bytes_le #U32 (sub result_block 0 4)) in
+  let j2 = uint_to_nat (uint_from_bytes_le #U32 (sub result_block 4 4)) in
+  let i' = if (r = 0 && j/4 = 0) then i else j2 % lanes in
+  let x = j1*$j1 / (pow2 32) in
+  let (first_available_block,available_blocks) =
+    (* All the blocks of the previous computed slices in selected lane, minus one if ours is first block of slice*)
+    if i' = j then
+      (* We select blocks in the same lane that we are computing *)
+      (0, slice*$segment_length - (if j%4 = 0 then 1 else 0))
+    else
+      (* We select blocks from a lane that we have already computed *)
+      (segment_length*$((slice+1) % 4), 3*$segment_length - (if j%4 = 0 then 1 else 0))
+  in
+  let y = (available_blocks*$x)/(pow2 32) in
+  let z = available_blocks - 1 - y in
+  let j' = (first_available_block + z) % columns in
+  (i',j')
+
+val step5 : iterations:size_nat -> t_len:size_nat{1 <= t_len /\ t_len <= block_size - 64} -> lanes:size_nat{lanes >= 1 /\ lanes <= pow2 24 - 1} -> columns:size_nat{4 <= columns /\ lanes*$columns*$block_size <= max_size_t} -> mem: lbytes (lanes*$columns*$block_size) -> Tot (lbytes (lanes*$columns*$block_size))
+
+let step5 iterations t_len lanes columns mem =
+  repeati lanes (fun i (mem: lbytes (lanes*$columns*$block_size)) ->
+    repeati (columns-1) (fun j (mem:lbytes (lanes*$columns*$block_size)) ->
       let j = j + 1 in
       let offset = block_offset lanes columns i j in
-      let first_block = sub mem (block_offset lanes columns i (j-1)) size_of_block in
-      let second_block = sub mem (block_offset lanes columns i j (*TODO*)) size_of_block in
+      let first_block = sub mem (block_offset lanes columns i (j-1)) block_size in
+      let i',j' = map_indexes iterations 1 lanes columns i j in
+      let second_block = sub mem (block_offset lanes columns i' j') block_size in
       let slice = argon_compress first_block second_block  in
-      update_slice mem offset (offset+ size_of_block) slice
+      update_slice mem offset (offset+ block_size) slice
     ) mem
   ) mem
 
+val step6 : iterations:size_nat -> t_len:size_nat{1 <= t_len /\ t_len <= block_size - 64} -> lanes:size_nat{lanes >= 1 /\ lanes <= pow2 24 - 1} -> columns:size_nat{4 <= columns /\ lanes*$columns*$block_size <= max_size_t} -> mem: lbytes (lanes*$columns*$block_size) -> Tot (lbytes (lanes*$columns*$block_size))
+
+#reset-options "--z3rlimit 500 --max_fuel 1"
+
+let step6 iterations t_len lanes columns mem =
+  if iterations <= 1 then mem else
+    repeati (iterations - 1) (fun r mem ->
+      let r = r + 1 in
+      repeati lanes (fun i (mem: lbytes (lanes*$columns*$block_size)) ->
+	repeati (columns-1) (fun j (mem:lbytes (lanes*$columns*$block_size)) ->
+	  let col_idx = if j = 0 then columns - 1 else j - 1 in
+	  let i',j' = map_indexes iterations r lanes columns i j in
+	  let arg1 : lbytes block_size = sub mem (block_offset lanes columns i j) block_size in
+	  let arg2 : lbytes block_size = argon_compress
+	     (sub mem (block_offset lanes columns i col_idx) block_size)
+	     (sub mem (block_offset lanes columns i' j') block_size)
+	  in
+	  let offset = block_offset lanes columns i j in
+	  update_slice mem offset (offset + block_size) (xor_matrices arg1 arg2)
+	) mem
+      ) mem
+    ) mem
+
+val step7 : lanes:size_nat{lanes >= 1 /\ lanes <= pow2 24 - 1} -> columns:size_nat{4 <= columns /\ lanes*$columns*$block_size <= max_size_t} ->  mem:lbytes (lanes*$columns*$block_size) -> Tot (lbytes block_size)
+
+let step7 lanes columns mem =
+  let block = sub mem (block_offset lanes columns 0 (columns - 1)) block_size in
+  repeati (lanes-1) (fun i block ->
+    let i = i + 1 in
+    xor_matrices block (sub mem (block_offset lanes columns i (columns - 1)) block_size)
+  ) block
 
 val argon2i :
   p_len:size_nat -> p : lbytes p_len ->
   s_len:size_nat{s_len >= 8} -> s: lbytes s_len ->
-  lanes:size_nat{lanes >= 1 /\ lanes <= pow2 24 - 1} -> t_len:size_nat{t_len >= 4 /\ t_len <= size_of_block - 64} ->
-  m:size_nat{m >= (8 * lanes) /\ (m + 4 * lanes)  * 1024 <= max_size_t} ->
+  lanes:size_nat{lanes >= 1 /\ lanes <= pow2 24 - 1} -> t_len:size_nat{t_len >= 4 /\ t_len <= block_size - 64} ->
+  m:size_nat{m >= (8*$lanes) /\ (m + 4*$lanes)*$1024 <= max_size_t} ->
   iterations:size_nat{iterations >= 1}  ->
-  x_len:size_nat{x_len + 4 <= max_size_t - 2 * Spec.Blake2b.bytes_in_block} -> x:lbytes x_len ->
-  k_len:size_nat{k_len + p_len + s_len + x_len + 11*4 <= max_size_t - 2 * Spec.Blake2b.bytes_in_block} -> k:lbytes k_len ->
-  Tot (lbytes t_len)
+  x_len:size_nat{x_len + 4 <= max_size_t - 2*$line_size} -> x:lbytes x_len ->
+  k_len:size_nat{k_len + p_len + s_len + x_len + 11*$4 <= max_size_t - 2 *$line_size} -> k:lbytes k_len ->
+  Tot (lbytes (compute_variable_length_output_size t_len))
 
 let argon2i p_len p s_len s lanes t_len m iterations x_len x k_len k =
   let h0 = step1 p_len p s_len s lanes t_len m iterations x_len x k_len k in
-  let four_lanes = 4 * lanes in
-  let columns = 4 * (m / four_lanes) in
-  let number_of_blocks = lanes * columns in
-  let memory_size : size_nat = size_of_block * number_of_blocks in
+  let four_lanes = 4*$lanes in
+  let columns = 4*$(m / four_lanes) in
+  let number_of_blocks = lanes*$columns in
+  let memory_size : size_nat = block_size*$number_of_blocks in
   let memory = create memory_size (u8 0) in
-  assert (memory_size = columns * lanes * size_of_block);
+  assert (memory_size = columns*$lanes*$block_size);
   let memory = step3 t_len lanes columns memory h0 in
   let memory = step4 t_len lanes columns memory h0 in
-  create t_len (u8 0)
+  let memory = step5 iterations t_len lanes columns memory in
+  let memory = step6 iterations t_len lanes columns memory in
+  let final_block = step7 lanes columns memory in
+  h' t_len block_size final_block
