specs/tests/Spec.Argon2i.Test.fst
@@ -1,0 +1,75 @@
+module Spec.Argon2i.Test
+
+#reset-options "--z3rlimit 100 --max_fuel 0"
+
+open FStar.Mul
+open Spec.Lib.IntTypes
+open Spec.Lib.RawIntTypes
+open Spec.Lib.IntSeq
+
+let password_list = List.Tot.map u8_from_UInt8 [
+  0x01uy; 0x01uy; 0x01uy; 0x01uy; 0x01uy; 0x01uy; 0x01uy; 0x01uy;
+  0x01uy; 0x01uy; 0x01uy; 0x01uy; 0x01uy; 0x01uy; 0x01uy; 0x01uy;
+  0x01uy; 0x01uy; 0x01uy; 0x01uy; 0x01uy; 0x01uy; 0x01uy; 0x01uy;
+  0x01uy; 0x01uy; 0x01uy; 0x01uy; 0x01uy; 0x01uy; 0x01uy; 0x01uy
+]
+
+let password : lbytes 32 = assert_norm (List.Tot.length password_list = 32);createL password_list
+
+let nonce_list = List.Tot.map u8_from_UInt8 [
+  0x02uy; 0x02uy; 0x02uy; 0x02uy; 0x02uy; 0x02uy; 0x02uy; 0x02uy;
+  0x02uy; 0x02uy; 0x02uy; 0x02uy; 0x02uy; 0x02uy; 0x02uy; 0x02uy
+]
+
+let nonce : lbytes 16 = assert_norm (List.Tot.length nonce_list = 16);createL nonce_list
+
+let key_list = List.Tot.map u8_from_UInt8 [
+  0x03uy; 0x03uy; 0x03uy; 0x03uy; 0x03uy; 0x03uy; 0x03uy; 0x03uy
+]
+
+let key : lbytes 8 = assert_norm (List.Tot.length key_list = 8);createL key_list
+
+let associated_data_list = List.Tot.map u8_from_UInt8 [
+  0x04uy; 0x04uy; 0x04uy; 0x04uy; 0x04uy; 0x04uy; 0x04uy; 0x04uy; 
+  0x04uy; 0x04uy; 0x04uy; 0x04uy
+]
+
+let associated_data : lbytes 12 = assert_norm (List.Tot.length associated_data_list = 12);
+  createL associated_data_list
+
+let expected_list = List.Tot.map u8_from_UInt8 [
+  0xc8uy; 0x14uy; 0xd9uy; 0xd1uy; 0xdcuy; 0x7fuy; 0x37uy; 0xaauy;
+  0x13uy; 0xf0uy; 0xd7uy; 0x7fuy; 0x24uy; 0x94uy; 0xbduy; 0xa1uy;
+  0xc8uy; 0xdeuy; 0x6buy; 0x01uy; 0x6duy; 0xd3uy; 0x88uy; 0xd2uy;
+  0x99uy; 0x52uy; 0xa4uy; 0xc4uy; 0x67uy; 0x2buy; 0x6cuy; 0xe8uy
+]
+
+let expected : lbytes 32 = assert_norm (List.Tot.length expected_list = 32); createL expected_list
+
+let test () =
+
+  IO.print_string "\nTEST 1\n";
+  let p_len = 32 in
+  let p = password in
+  let s_len = 16 in
+  let s = nonce in
+  let lanes = 4 in
+  let t_len = 32 in
+  let m = 32 in
+  let iterations = 3 in
+  let x_len = 12 in
+  let x = associated_data in
+  let k_len = 8 in
+  let k = key in
+  let output : lbytes 32 =
+    Spec.Argon2i.argon2i p_len p s_len s lanes t_len m iterations x_len x k_len k 
+  in
+  let result = for_all2 (fun a b -> uint_to_nat #U8 a = uint_to_nat #U8 b) expected output in
+  IO.print_string "\nResult   ARGON2i: ";
+  List.iter (fun a -> IO.print_string (UInt8.to_string (u8_to_UInt8 a))) (as_list output);
+
+  IO.print_string "\nExpected ARGON2i: ";
+  List.iter (fun a -> IO.print_string (UInt8.to_string (u8_to_UInt8 a))) (as_list expected);
+
+  if result then IO.print_string "\nARGON2i Test1 : Success!\n"
+  else IO.print_string "\nARGON2i Test1: Failure :(\n"
